*PHFFP p. 635*

This is good
```haskell
data CountingGood a = Heisenberg Int a deriving (Eq, Show)

instance Functor CountingGood where
  fmap :: (a -> b) -> CountingGood a -> CountingGood b
  fmap f (Heisenberg n a) = Heisenberg n (f a)
```

This isn't because it changes the first argument to `Heisenberg` and `fmap` should only change the last one.
> But what if a type had 3 arguments line `Something a b c`. Should `fmap` change the `b` or `c`.

```haskell
instance Functor CountingBad where
  fmap :: (a -> b) -> CountingBad a -> CountingBad b
  fmap f (Heisenberg n a) = Heisenberg (n+1) (f a)
```

The bad outcome here is that `fmap (f . g)` will not equal `fmap f . fmap g` because the former with one `fmap` will increment `n` once but the latter with two `fmap`'s will increment `n` twice.
