
This works
```haskell
data FixMePls a = FixMe | Pls a deriving (Eq, Show)

instance Functor FixMePls where -- [A]
  fmap _ FixMe = FixMe
  fmap f (Pls a) = Pls (f a)
```

This doesn't
```haskell

data FixMePls a = FixMe | Pls a deriving (Eq, Show)

instance Functor (FixMePls a) where -- [B]
  fmap _ FixMe = FixMe
  fmap f (Pls a) = Pls (f a)
```

```haskell
• Expected kind ‘* -> *’, but ‘FixMePls a’ has 
  kind ‘*’  
• In the first argument of ‘Functor’, namely 
  ‘(FixMePls a)’  
  In the instance declaration for ‘Functor 
  (FixMePls a)’
```

Putting `(FixMePls a)` in `()` makes it part of the type structure and it is no longer an argument to the data constructor.
