# #monad

#monad

## What's different about `>>=`


```haskell
fmap :: Functor     f =>   (a -> b) -> f a -> f b
<*>  :: Applicative f => f (a -> b) -> f a -> f b
>>= ::  Monad       f => f a -> (a -> f b) -> f b
```

`>>=` ("bind") is quite similar to `<*>` and `fmap` but with the first two arguments flipped

Here they are flipped (which means `fmap` & `<*>*` are not valid) 
```haskell
fmap :: Functor     f => f a ->   (a -> b) -> f b
<*>  :: Applicative f => f a -> f (a -> b) -> f b
>>= ::  Monad       f => f a -> (a -> f b) -> f b
```

If I give `fmap` a function `(a -> f b)` which is what `>>=` takes, it will produce a nested structure

While `<*>` & `<$>` leave structure alone they can result in nested structures, `>>=` will not.

`>>=` combines `join` with `fmap`
```haskell
join :: Monad m => m (m a) -> m a
```

So `Monad` is much like `Functor` & `Applicative` but it has the `join` function. Where `<$>` & `<*>` can create nested structures, `>>=` uses `join` to keep the structure flat.

> [!INFO] `lift`
> The Monad `liftM*` functions don't do anything different than `Monad` but they are around because some libraries still use them.


## `join` is like `concat`

`concat`
```haskell
concat :: Foldable t => t [a] -> [a]
```
could be writing specifically for `[]`
```haskell
concat :: [[a]] -> [a]
```
and `join` is
```haskell
join :: Monad m => m (m a) -> m a
```
Both are removing some structure. Example:
```haskell
b = fmap addOne [4,5,6]
-- [[4,1],[5,1],[6,1]]
c = join $ fmap addOne [4,5,6]
-- [4,1,5,1,6,1]
d = concat $ fmap addOne [4,5,6]
-- [4,1,5,1,6,1]
```
In this case, `join` and `concat` do the same thing.


### When `fmap` alone isn't enough

g :: (String -> b) -> IO b
g x = x <$> getLine

z :: IO ()
z = join $ putStrLn <$> getLine :: IO ()


Mapping `putStrLn` over `getLine` results in an `IO` inside an `IO`. If you run it nothing is printed.
```haskell
> :t putStrLn <$> getLine
putStrLn <$> getLine :: IO (IO ()) -- IO in a IO
> putStrLn <$> getLine
kk
>
-- there is no output
```

The solution is to join them which solves the problem.
```haskell
> :t join $ putStrLn <$> getLine
join $ putStrLn <$> getLine :: IO () -- an IO ()

> join $ putStrLn <$> getLine
kk
kk -- the output
>
```

Mapping `putStrLn` over a `Functor` results in an `IO` in a `Functor`.
```haskell
> b x = putStrLn <$> x
> :t b (Just "h")
b (Just "h") :: Maybe (IO ())
```


### Example of the list monad in use:
```haskell
twiceWhenEven :: [Integer] -> [Integer]
twiceWhenEven xs = do
  x <- xs                            -- [A], [B]
  if even x
  then [x*x, x*x]
  else [x*x]
```
- $[A]$ Yep, like a list comprehension it sends the values of the list one by one
- $[B]$ (>>=) :: [a] -> (a -> [b]) -> [b] -- is this the right signature
    - - [a] is xs
    - - the `if` is (a -> [b])

With regard to Monads:
- 

```haskell
twiceWhenEven' :: [Integer] -> [Integer]
twiceWhenEven' xs = do
  x <- xs
  if even x
  then [x*x, x*x]
  else []

> twiceWhenEven' [1,2,3]
[4,4]
```



As a list comprehension
```haskell
e :: [[Integer]]
e = [ k | i <- [1..3], let k = (if even (i*i) then [i*i, i*i] else [i*i] )]

> e
[[1],[4,4],[9]]
```
Actually, I got that wrong, the answer should be `[1,4,4,9]`. I tried to find a way to keep it all inside of the list comprehension but didn't find one. Therefore have used `mconcat` outside.
```haskell
f :: Integral t => [t] -> [t]
f xs = mconcat [ k | i <- xs, let k = (if even (i*i) then [i*i, i*i] else [i*i] )]
```


There is lots of interesting stuff going on in the above example. In regards to Monads

```haskell
(>>=) :: Monad m => m  a -> (a -> m b) -> m b

```



## Maybe Monad

```haskell
(>>=) :: Monad m => m a -> (a -> m b) ->         m b
(>>=) ::        Maybe a -> (a -> Maybe b) -> Maybe b
```


## Either Monad
![[haskell-notes/Pasted image 20220817121343.png]]
*Had to past a picture here bec the text version wrapped :(*

So I take it that `a` gets transformed to `b` , but the `e` never will be changed.


## Random Stuff

Write `fmap` using monadic operations
```haskell
fmap f xs = xs >>= return . f
```

This could go on forever
```haskell
m a  -> (a -> m a) -> (a -> ma)
```

## ?
```haskell
(>>=) :: forall a b. m a -> (a -> m b) -> m b
(>=>) :: Monad m => (a -> m b) -> (b -> m c) -> a -> m c 

(>>=) :: m a -> (a -> m b) -> m b
(>=>) :: Monad m => (a -> m b) -> (b -> m c) -> a -> m c
```

```haskell
(>>=) :: m a -> (a -> m b) -> m b
(>=>) :: (a -> m b) -> (b -> m c) -> a -> m c 
```