

Given:

```haskell
data Box a = Box a deriving Show

instance Functor Box where
fmap func (Box val) = Box (func val)

myBox :: Box Int
myBox = Box 1
```

1. use `fmap` to put your `myBox` into another `Box`.
2. Then write a function `unwrap` that takes a value out of a box and use `fmap`  on that function to get the original box.

Here is how it should work in GHCi
```haskell
GHCi> wrapped = fmap ? myBox
GHCi> wrapped
Box (Box 1)
GHCi> fmap unwrap wrapped
Box 1
```

Books solution

```haskell
myBox :: Box Int
myBox = Box 1

unwrap :: Box a -> a
unwrap (Box val) = val
```

But `fmap` isn't needed. So is the author just trying to make a point that I'm not seeing?